Turned list_sort generic, so the service takes compare in protocol

theories/examples/list_sort.v
@@ -11,221 +11,238 @@ Require Import Omega.
 Section ListSortExample.
   Context `{!heapG Σ} `{logrelG val Σ} (N : namespace).
 
-  Definition lsplit_ref : val :=
-    λ: "xs", let: "ys_zs" := lsplit !"xs" in
-             (ref (Fst "ys_zs"), ref (Snd ("ys_zs"))).
+  Section SortService.
+    Context `{EncDec T}.
+    Context (R : relation T) `{!Total R} `{∀ x y, Decision (R x y)}.
 
-  Lemma lsplit_ref_spec lxs (x : Z) (xs : list Z) :
-    {{{ lxs ↦ encode (x::xs) }}}
-      lsplit_ref #lxs
-    {{{ lys lzs ys zs, RET (#lys,#lzs);
-        ⌜(x::xs) = ys++zs⌝ ∗
-        lxs ↦ encode (x::xs) ∗
-        lys ↦ encode ys ∗
-        lzs ↦ encode zs }}}.
-  Proof.
-    iIntros (Φ) "Hhd HΦ".
-    wp_lam. wp_load. wp_apply (lsplit_spec (T:=Z))=> //. iIntros (ys zs <-).
-    wp_alloc lzs as "Hlzs".
-    wp_alloc lys as "Hlys".
-    wp_pures.
-    iApply "HΦ".
-    eauto 10 with iFrame.
-  Qed.
+    Definition lsplit_ref : val :=
+      λ: "xs", let: "ys_zs" := lsplit !"xs" in
+               (ref (Fst "ys_zs"), ref (Snd ("ys_zs"))).
+
+    Lemma lsplit_ref_spec lxs (x : T) (xs : list T) :
+      {{{ lxs ↦ encode (x::xs) }}}
+        lsplit_ref #lxs
+      {{{ lys lzs ys zs, RET (#lys,#lzs);
+          ⌜(x::xs) = ys++zs⌝ ∗
+                       lxs ↦ encode (x::xs) ∗
+                       lys ↦ encode ys ∗
+                       lzs ↦ encode zs }}}.
+    Proof.
+      iIntros (Φ) "Hhd HΦ".
+      wp_lam. wp_load. wp_apply (lsplit_spec)=> //. iIntros (ys zs <-).
+      wp_alloc lzs as "Hlzs".
+      wp_alloc lys as "Hlys".
+      wp_pures.
+      iApply "HΦ".
+      eauto 10 with iFrame.
+    Qed.
+
+    Definition lmerge : val :=
+      rec: "go" "cmp" "hys" "hzs" :=
+        match: "hys" with
+          NONE => "hzs"
+        | SOME "_" =>
+          match: "hzs" with
+            NONE => "hys"
+          | SOME "_" =>
+            let: "y" := lhead "hys" in
+            let: "z" := lhead "hzs" in
+            if: ("cmp" "y" "z")
+            then lcons "y" ("go" "cmp" (ltail "hys") "hzs")
+            else lcons "z" ("go" "cmp" "hys" (ltail "hzs"))
+          end
+        end.
+
+    Lemma list_merge_emp1 (ys : list T) : list_merge (R) [] ys = ys.
+    Proof. induction ys; eauto. Qed.
+
+    Lemma list_merge_emp2 (xs : list T) : list_merge (R) xs [] = xs.
+    Proof. induction xs; eauto. Qed.
+
+    Definition cmp_spec (cmp : val) : iProp Σ :=
+      (∀ x y, {{{ True }}}
+                cmp (encode x) (encode y)
+              {{{ RET encode (bool_decide (R x y)); True}}})%I.
+
+    Lemma lmerge_spec  (cmp : val) (ys zs : list T) :
+      cmp_spec cmp →
+      {{{ True }}}
+        lmerge cmp (encode ys) (encode zs)
+      {{{ RET (encode (list_merge (R) ys zs)); True }}}.
+    Proof.
+      revert ys zs.
+      iLöb as "IH".
+      iIntros (ys zs Hcmp_spec Φ _) "HΦ".
+      wp_lam.
+      destruct ys as [|y ys].
+      { wp_pures. rewrite list_merge_emp1. by iApply ("HΦ"). }
+      destruct zs as [|z zs].
+      { wp_pures. rewrite list_merge_emp2. by iApply ("HΦ"). }
+      wp_apply (lhead_spec)=> //; iIntros "_".
+      wp_apply (lhead_spec)=> //; iIntros "_".
+      wp_apply (Hcmp_spec)=> //; iIntros "_".
+      rewrite list_merge_cons.
+      destruct (decide (R y z)).
+      - rewrite bool_decide_true=> //.
+        wp_apply (ltail_spec)=> //; iIntros (_).
+        wp_apply ("IH")=> //; iIntros (_).
+        wp_apply (lcons_spec)=> //.
+      - rewrite bool_decide_false=> //.
+        wp_apply (ltail_spec)=> //; iIntros (_).
+        wp_apply ("IH")=> //; iIntros (_).
+        wp_apply (lcons_spec)=> //.
+    Qed.
+
+    Definition lmerge_ref : val :=
+      λ: "cmp" "lxs" "hys" "hzs",
+      "lxs" <- lmerge "cmp" "hys" "hzs".
+
+    Lemma lmerge_ref_spec (cmp : val) ldx tmp ys zs :
+      cmp_spec cmp →
+      {{{ ldx ↦ tmp }}}
+        lmerge_ref cmp #ldx (encode ys) (encode zs)
+      {{{ RET #(); ldx ↦ encode (list_merge R ys zs) }}}.
+    Proof.
+      iIntros (cmp_spec Φ) "Hldx HΦ".
+      wp_lam.
+      wp_apply (lmerge_spec cmp ys zs)=> //.
+      iIntros (_).
+      wp_store.
+      by iApply ("HΦ").
+    Qed.
+
+    Definition list_sort_service : val :=
+      rec: "go" "c" :=
+        let: "cmp" := recv "c" #Right in
+        let: "xs" := recv "c" #Right in
+        if: llength (!"xs") ≤ #1
+        then send "c" #Right "xs"
+        else let: "ys_zs" := lsplit_ref "xs" in
+             let: "ys" := Fst "ys_zs" in
+             let: "zs" := Snd "ys_zs" in
+             let: "cy" := new_chan #() in Fork("go" "cy");;
+             let: "cz" := new_chan #() in Fork("go" "cz");;
+             send "cy" #Left "cmp";;
+             send "cy" #Left "ys";;
+             send "cz" #Left "cmp";;
+             send "cz" #Left "zs";;
+             let: "ys" := recv "cy" #Left in
+             let: "zs" := recv "cz" #Left in
+             lmerge_ref "cmp" "xs" !"ys" !"zs";;
+             send "c" #Right "xs".
+
+    Definition sort_protocol xs :=
+      (<?> cmp @ ⌜cmp_spec cmp⌝,
+       <?> l @ l ↦ encode xs,
+       <!> l' @ ⌜l = l'⌝ ∗
+                (∃ ys : list T,
+                    l' ↦ encode ys ∗
+                       ⌜Sorted (R) ys⌝ ∗
+                       ⌜Permutation ys xs⌝),
+       TEnd)%stype.
+
+    Lemma list_sort_service_spec γ c xs :
+      {{{ ⟦ c @ Right : sort_protocol xs ⟧{N,γ} }}}
+        list_sort_service c
+      {{{ RET #(); ⟦ c @ Right : TEnd ⟧{N,γ} }}}.
+    Proof.
+      revert γ c xs.
+      iLöb as "IH".
+      iIntros (γ c xs Φ) "Hstr HΦ".
+      wp_lam.
+      wp_apply (recv_st_spec N val with "Hstr").
+      iIntros (cmp) "[Hstr cmp_spec]".
+      iDestruct ("cmp_spec") as %Hcmp_spec.
+      wp_pures.
+      wp_apply (recv_st_spec N loc with "Hstr").
+      iIntros (v) "Hstr".
+      iDestruct "Hstr" as "[Hstr HP]".
+      wp_load.
+      destruct xs.
+      {
+        wp_apply (llength_spec)=> //; iIntros (_).
+        wp_apply (send_st_spec N loc with "[HP Hstr]")=> //. iFrame.
+        eauto 10 with iFrame.
+      }
+      destruct xs.
+      {
+        wp_apply (llength_spec)=> //; iIntros (_).
+        wp_apply (send_st_spec N loc with "[HP Hstr]")=> //. iFrame.
+        eauto 10 with iFrame.
+      }
+      wp_apply (llength_spec)=> //; iIntros (_).
+      wp_pures.
+      assert (bool_decide (S (S (length xs)) ≤ 1) = false) as HSS.
+      { apply bool_decide_false. lia. }
+      rewrite HSS.
+      wp_apply (lsplit_ref_spec with "HP");
+        iIntros (hdy hdz ys zs) "(Heq & Hhdx & Hhdy & Hhdz)".
+      iDestruct "Heq" as %->.
+      wp_apply (new_chan_st_spec N _ (sort_protocol ys))=> //.
+      iIntros (cy γy) "[Hstly Hstry]".
+      wp_apply (wp_fork with "[Hstry]").
+      { iNext. iApply ("IH" with "Hstry"). iNext. by iIntros "Hstry". }
+      wp_apply (new_chan_st_spec N _ (sort_protocol zs))=> //.
+      iIntros (cz γz) "[Hstlz Hstrz]".
+      wp_apply (wp_fork with "[Hstrz]").
+      { iNext. iApply ("IH" with "Hstrz"). iNext. by iIntros "Hstrz". }
+      wp_apply (send_st_spec N val with "[Hstly]"). iFrame. done.
+      iIntros "Hstly".
+      wp_apply (send_st_spec N loc with "[Hhdy Hstly]"). iFrame.
+      iIntros "Hstly".
+      wp_apply (send_st_spec N val with "[Hstlz]"). iFrame. done.
+      iIntros "Hstlz".
+      wp_apply (send_st_spec N loc with "[Hhdz Hstlz]"). iFrame.
+      iIntros "Hstlz".
+      wp_apply (recv_st_spec N loc with "Hstly").
+      iIntros (ly') "[Hstly Hys']".
+      iDestruct "Hys'" as (<- ys') "(Hys' & Hys'_sorted_of)".
+      iDestruct "Hys'_sorted_of" as %[Hys'_sorted Hys'_perm].
+      wp_apply (recv_st_spec N loc with "Hstlz").
+      iIntros (lz') "[Hstlz Hzs']".
+      iDestruct "Hzs'" as (<- zs') "(Hzs' & Hzs'_sorted_of)".
+      iDestruct "Hzs'_sorted_of" as %[Hzs'_sorted Hzs'_perm].
+      wp_load.
+      wp_load.
+      wp_pures.
+      wp_apply (lmerge_ref_spec with "[Hhdx]")=> //.
+      iIntros "Hhdx".
+      wp_apply (send_st_spec N loc with "[Hstr Hhdx]").
+      {
+        iFrame.
+        iSplit=> //.
+        iExists (list_merge R ys' zs').
+        iSplit=> //.
+        iPureIntro.
+        split.
+        - apply Sorted_list_merge=> //.
+        - rewrite merge_Permutation.
+            by apply Permutation_app.
+      }
+      iIntros "Hstr".
+      by iApply "HΦ".
+    Qed.
+  End SortService.
 
   Definition compare_vals : val :=
     λ: "x" "y", "x" ≤ "y".
+
+  Instance total_le : Total Z.le.
+  Proof. intros x y. lia. Qed.
 
   Lemma compare_vals_spec (x y : Z) :
     {{{ True }}}
       compare_vals (encode x) (encode y)
     {{{ RET (encode (bool_decide (x ≤ y))); True }}}.
   Proof. iIntros (Φ) "_ HΦ". wp_lam. wp_pures. by iApply "HΦ". Qed.
-    
-  Definition lmerge : val :=
-    rec: "go" "hys" "hzs" :=
-      match: "hys" with
-        NONE => "hzs"
-      | SOME "_" =>
-        match: "hzs" with
-          NONE => "hys"
-        | SOME "_" =>
-          let: "y" := lhead "hys" in
-          let: "z" := lhead "hzs" in
-          if: (compare_vals "y" "z")
-          then lcons "y" ("go" (ltail "hys") "hzs")
-          else lcons "z" ("go" "hys" (ltail "hzs"))
-        end
-      end.
-
-  Lemma list_merge_emp1 (ys : list Z) : list_merge (≤) [] ys = ys.
-  Proof. induction ys; eauto. Qed.
-
-  Lemma list_merge_emp2 (xs : list Z) : list_merge (≤) xs [] = xs.
-  Proof. induction xs; eauto. Qed.
-
-  Lemma lmerge_spec (ys zs : list Z) :
-    {{{ True }}}
-      lmerge (encode ys) (encode zs)
-    {{{ RET (encode (list_merge (≤) ys zs)); True }}}.
-  Proof.
-    revert ys zs.
-    iLöb as "IH".
-    iIntros (ys zs Φ _) "HΦ".
-    wp_lam.
-    destruct ys as [|y ys].
-    { wp_pures. rewrite list_merge_emp1. by iApply ("HΦ"). }
-    destruct zs as [|z zs].
-    { wp_pures. rewrite list_merge_emp2. by iApply ("HΦ"). }
-    wp_apply (lhead_spec (T:=Z))=> //; iIntros "_".
-    wp_apply (lhead_spec (T:=Z))=> //; iIntros "_".
-    wp_apply (compare_vals_spec)=> //; iIntros "_".
-    rewrite list_merge_cons.
-    destruct (decide (y ≤ z)).
-    - rewrite bool_decide_true=> //.
-      wp_apply (ltail_spec (T:=Z))=> //; iIntros (_).
-      wp_apply ("IH")=> //; iIntros (_).
-      wp_apply (lcons_spec (T:=Z))=> //.
-    - rewrite bool_decide_false=> //.
-      wp_apply (ltail_spec (T:=Z))=> //; iIntros (_).
-      wp_apply ("IH")=> //; iIntros (_).
-      wp_apply (lcons_spec (T:=Z))=> //.
-  Qed.
-
-  Definition lmerge_ref : val :=
-    λ: "lxs" "hys" "hzs",
-      "lxs" <- lmerge "hys" "hzs".
-
-  Lemma lmerge_ref_spec ldx tmp ys zs :
-    {{{ ldx ↦ tmp }}}
-      lmerge_ref #ldx (encode ys) (encode zs)
-    {{{ RET #(); ldx ↦ encode (list_merge (≤) ys zs) }}}.
-  Proof.
-    iIntros (Φ) "Hldx HΦ".
-    wp_lam.
-    wp_apply (lmerge_spec ys zs)=> //.
-    iIntros (_).
-    wp_store.
-    by iApply ("HΦ").
-  Qed.
-
-  Definition list_sort_service : val :=
-    rec: "go" "c" :=
-      let: "xs" := recv "c" #Right in
-      if: llength (!"xs") ≤ #1
-      then send "c" #Right "xs"
-      else let: "ys_zs" := lsplit_ref "xs" in
-           let: "ys" := Fst "ys_zs" in
-           let: "zs" := Snd "ys_zs" in
-           let: "cy" := new_chan #() in Fork("go" "cy");;
-           let: "cz" := new_chan #() in Fork("go" "cz");;
-           send "cy" #Left "ys";;
-           send "cz" #Left "zs";;
-           let: "ys" := recv "cy" #Left in
-           let: "zs" := recv "cz" #Left in
-           lmerge_ref "xs" !"ys" !"zs";;
-           send "c" #Right "xs".
-
-  Lemma list_sort_service_spec γ c xs :
-    {{{ ⟦ c @ Right : (<?> l @ l ↦ encode xs,
-                          <!> l' @
-                          ⌜l = l'⌝ ∗ (∃ ys : list Z,
-                                      l' ↦ encode ys ∗
-                                      ⌜Sorted (≤) ys⌝ ∗
-                                      ⌜Permutation ys xs⌝),
-                          TEnd) ⟧{N,γ} }}}
-      list_sort_service c
-    {{{ RET #(); ⟦ c @ Right : TEnd ⟧{N,γ} }}}.
-  Proof.
-    revert γ c xs.
-    iLöb as "IH".
-    iIntros (γ c xs Φ) "Hstr HΦ".
-    wp_lam.
-    wp_apply (recv_st_spec N loc with "Hstr").
-    iIntros (v) "Hstr".
-    iDestruct "Hstr" as "[Hstr HP]".
-    wp_load.
-    destruct xs.
-    {
-      wp_apply (llength_spec (T:=Z))=> //; iIntros (_).
-      wp_apply (send_st_spec N loc with "[HP Hstr]")=> //. iFrame.
-      eauto 10 with iFrame.
-    }
-    destruct xs.
-    {
-      wp_apply (llength_spec (T:=Z))=> //; iIntros (_).
-      wp_apply (send_st_spec N loc with "[HP Hstr]")=> //. iFrame.
-      eauto 10 with iFrame.
-    }
-    wp_apply (llength_spec (T:=Z))=> //; iIntros (_).
-    wp_pures.
-    assert (bool_decide (S (S (length xs)) ≤ 1) = false) as HSS.
-    { apply bool_decide_false. lia. }
-    rewrite HSS.
-    wp_apply (lsplit_ref_spec with "HP");
-      iIntros (hdy hdz ys zs) "(Heq & Hhdx & Hhdy & Hhdz)".
-    iDestruct "Heq" as %->.
-    wp_apply (new_chan_st_spec N
-               (<!> l @ l ↦ encode ys,
-                <?> l' @ ⌜l = l'⌝ ∗
-                         (∃ ys' : list Z,
-                             l' ↦ encode ys' ∗
-                                ⌜Sorted (≤) ys'⌝ ∗
-                                ⌜Permutation ys' ys⌝),
-                TEnd))=>//;
-             iIntros (cy γy) "[Hstly Hstry]".
-    wp_apply (wp_fork with "[Hstry]").
-    { iNext. iApply ("IH" with "Hstry"). iNext. by iIntros "Hstry". }
-    wp_apply (new_chan_st_spec N
-               (<!> l @ l ↦ encode zs,
-                <?> l' @ ⌜l = l'⌝ ∗
-                         (∃ zs' : list Z,
-                             l' ↦ encode zs' ∗
-                                ⌜Sorted (≤) zs'⌝ ∗
-                                ⌜Permutation zs' zs⌝),
-                TEnd))=>//;
-    iIntros (cz γz) "[Hstlz Hstrz]".
-    wp_apply (wp_fork with "[Hstrz]").
-    { iNext. iApply ("IH" with "Hstrz"). iNext. by iIntros "Hstrz". }
-    wp_apply (send_st_spec N loc with "[Hhdy Hstly]"). iFrame.
-    iIntros "Hstly".
-    wp_apply (send_st_spec N loc with "[Hhdz Hstlz]"). iFrame.
-    iIntros "Hstlz".
-    wp_apply (recv_st_spec N loc with "Hstly").
-    iIntros (ly') "[Hstly Hys']".
-    iDestruct "Hys'" as (<- ys') "(Hys' & Hys'_sorted_of)".
-    iDestruct "Hys'_sorted_of" as %[Hys'_sorted Hys'_perm].
-    wp_apply (recv_st_spec N loc with "Hstlz").
-    iIntros (lz') "[Hstlz Hzs']".
-    iDestruct "Hzs'" as (<- zs') "(Hzs' & Hzs'_sorted_of)".
-    iDestruct "Hzs'_sorted_of" as %[Hzs'_sorted Hzs'_perm].
-    wp_load.
-    wp_load.
-    wp_apply (lmerge_ref_spec with "Hhdx")=> //.
-    iIntros "Hhdx".
-    wp_apply (send_st_spec N loc with "[Hstr Hhdx]").
-    {
-      iFrame.
-      iSplit=> //.
-      iExists (list_merge (≤) ys' zs').
-      iSplit=> //.
-      iPureIntro.
-      split.
-      - apply Sorted_list_merge=> //.
-        { intros x y. lia. }    (* Why is this needed? *)
-      - rewrite merge_Permutation.
-        by apply Permutation_app.
-    }
-    iIntros "Hstr".
-    by iApply "HΦ".
-  Qed.
 
   Definition list_sort : val :=
     λ: "xs",
     let: "c" := new_chan #() in
     Fork(list_sort_service "c");;
-    send "c" #Left "xs";;
-    recv "c" #Left.
+        send "c" #Left compare_vals;;
+        send "c" #Left "xs";;
+        recv "c" #Left.
 
   Lemma list_sort_spec l xs :
     {{{ l ↦ encode xs }}}
@@ -234,19 +251,30 @@ Section ListSortExample.
   Proof.
      iIntros (Φ) "Hc HΦ".
      wp_lam.
-     wp_apply (new_chan_st_spec N
-                 (<!> l @ l ↦ encode xs,
-                  <?> l' @ ⌜l = l'⌝ ∗
-                           (∃ ys : list Z,
-                               l' ↦ encode ys ∗
-                                  ⌜Sorted (≤) ys⌝ ∗
-                                  ⌜Permutation ys xs⌝), TEnd))=>//.
+     wp_apply (new_chan_st_spec N _ (sort_protocol (≤) xs))=> //.
      iIntros (c γ) "[Hstl Hstr]".
      wp_apply (wp_fork with "[Hstr]").
      {
-       iApply (list_sort_service_spec γ c xs with "[Hstr]"). iFrame.
+       iApply (list_sort_service_spec (≤) γ c xs with "Hstr").
        iNext. iNext. iIntros "Hstr". done.
      }
+     wp_apply (send_st_spec N val with "[$Hstl]").
+     {
+       iPureIntro.
+       iIntros (x y Φ').
+       iModIntro. iIntros (_) "HΦ".
+       iApply compare_vals_spec=> //.
+       iNext.
+       iIntros (_).
+       destruct (decide (x ≤ y)).
+       - rewrite bool_decide_true=>//.
+         rewrite bool_decide_true=>//.
+         by iApply "HΦ".
+       - rewrite bool_decide_false=>//.
+         rewrite bool_decide_false=>//.
+         by iApply "HΦ".
+     }
+     iIntros "Hstl".
      wp_apply (send_st_spec N loc with "[Hc $Hstl]"). iFrame.
      iIntros "Hstl".
      wp_apply (recv_st_spec N loc with "Hstl").
@@ -254,5 +282,4 @@ Section ListSortExample.
      iDestruct "HP" as (<- ys) "[Hys Hys_sorted_of]".
      iApply "HΦ". iFrame.
   Qed.
-
 End ListSortExample.
